src/program_proof/obj/recovery_proof.v
@@ -64,7 +64,7 @@ Definition block0_map : gmap u64 object :=
   {[W64 0 := existT _ (bufBlock block0)]}.
 
 Definition kind_heap0 (kinds: gmap u64 bufDataKind) : gmap addr object :=
-  map_uncurry (M1:=gmap _) (M2:=gmap _) ((λ K, match K with
+  map_uncurry ((λ K, match K with
                    | KindBit => bit0_map
                    | KindInode => inode0_map
                    | KindBlock => block0_map
@@ -465,6 +465,7 @@ Proof.
 
     rewrite /kind_heap0 /gmap_addr_by_block.
     rewrite map_curry_uncurry_non_empty; last first.
+    rewrite map_curry_uncurry_non_empty; last first.
     {
       intros i x Hix. rewrite lookup_fmap in Hix.
       apply fmap_Some_1 in Hix. destruct Hix. intuition idtac.
@@ -518,6 +519,7 @@ Proof.
     rewrite /bufDataTs_in_crashblock.
 
     rewrite /kind_heap0 /gmap_addr_by_block.
+    rewrite map_curry_uncurry_non_empty; last first.
     rewrite map_curry_uncurry_non_empty; last first.
     {
       intros i x Hix. rewrite lookup_fmap in Hix.
